fix by review

Logic/Propositional/Intuitionistic/Deduction.lean
@@ -8,7 +8,7 @@ variable {α : Type u} [DecidableEq α]
 inductive Deduction : Theory α → Formula α → Type _
   | axm {Γ p}                : p ∈ Γ → Deduction Γ p
   /-- **Remark**: This is stronger version. -/
-  | modus_ponens {Γ p q} : Deduction Γ (p ⟶ q) → Deduction Γ p → Deduction Γ q
+  | modusPonens {Γ p q} : Deduction Γ (p ⟶ q) → Deduction Γ p → Deduction Γ q
   | verum Γ          : Deduction Γ ⊤
   | imply₁ Γ p q     : Deduction Γ (p ⟶ q ⟶ p)
   | imply₂ Γ p q r   : Deduction Γ ((p ⟶ q ⟶ r) ⟶ (p ⟶ q) ⟶ p ⟶ r)
@@ -35,13 +35,15 @@ abbrev Theory.Inconsistent := Hilbert.Inconsistent (@Deduction α) Γ
 
 namespace Deduction
 
+open Hilbert
+
 variable {Γ : Theory α} {p q : Formula α}
 
 def weakening' {Γ Δ} {p : Formula α} (hs : Γ ⊆ Δ) : (Γ ⊢ᴵ p) → (Δ ⊢ᴵ p)
   | axm h => axm (hs h)
-  | modus_ponens h₁ h₂ => by
+  | modusPonens h₁ h₂ => by
       -- simp [Finset.union_subset_iff] at hs;
-      simpa using (h₁.weakening' hs).modus_ponens (h₂.weakening' hs);
+      simpa using (h₁.weakening' hs).modusPonens (h₂.weakening' hs);
   | verum _ => by apply verum
   | imply₁ _ _ _ => by apply imply₁
   | imply₂ _ _ _ _ => by apply imply₂
@@ -60,7 +62,7 @@ instance : Hilbert.Intuitionistic (@Deduction α) where
     rename_i Γ₁ Γ₂ p q
     replace h₁ : (Γ₁ ∪ Γ₂) ⊢ᴵ p ⟶ q := h₁.weakening' (by simp);
     replace h₂ : (Γ₁ ∪ Γ₂) ⊢ᴵ p := h₂.weakening' (by simp);
-    exact modus_ponens h₁ h₂;
+    exact modusPonens h₁ h₂;
   verum        := verum;
   imply₁       := imply₁;
   imply₂       := imply₂;
@@ -71,8 +73,6 @@ instance : Hilbert.Intuitionistic (@Deduction α) where
   disj₂        := disj₂;
   disj₃        := disj₃;
   efq          := efq
-
-def modus_ponens' {Γ : Theory α} {p q} : (Γ ⊢ᴵ (p ⟶ q)) → (Γ ⊢ᴵ p) → (Γ ⊢ᴵ q) := Hilbert.modus_ponens'
 
 private def dtrAux (Γ : Theory α) (p q) : (Γ ⊢ᴵ q) → ((Γ \ {p}) ⊢ᴵ (p ⟶ q))
   | verum _         => modus_ponens' (imply₁ _ _ _) (verum _)
@@ -92,13 +92,13 @@ private def dtrAux (Γ : Theory α) (p q) : (Γ ⊢ᴵ q) → ((Γ \ {p}) ⊢ᴵ
     case neg =>
       have d₁ : (Γ \ {p}) ⊢ᴵ (q ⟶ p ⟶ q) := imply₁ _ q p
       have d₂ : (Γ \ {p}) ⊢ᴵ q := axm (Set.mem_diff_singleton.mpr ⟨ih, Ne.symm h⟩)
-      exact d₁.modus_ponens' d₂;
-  | @modus_ponens _ Γ a b h₁ h₂ =>
+      exact modus_ponens' d₁ d₂;
+  | @modusPonens _ Γ a b h₁ h₂ =>
       have ih₁ : Γ \ {p} ⊢ᴵ p ⟶ a ⟶ b := dtrAux Γ p (a ⟶ b) h₁
       have ih₂ : Γ \ {p} ⊢ᴵ p ⟶ a := dtrAux Γ p a h₂
-      have d₁ : ((Γ) \ {p}) ⊢ᴵ (p ⟶ a) ⟶ p ⟶ b := (imply₂ _ p a b).modus_ponens' ih₁ |>.weakening' (by simp)
+      have d₁ : ((Γ) \ {p}) ⊢ᴵ (p ⟶ a) ⟶ p ⟶ b := modus_ponens' (imply₂ _ p a b) ih₁ |>.weakening' (by simp)
       have d₂ : ((Γ) \ {p}) ⊢ᴵ (p ⟶ a) := ih₂.weakening' (by simp)
-      d₁.modus_ponens' d₂
+      modus_ponens' d₁ d₂
 
 def dtr {Γ : Theory α} {p q} (d : (insert p Γ) ⊢ᴵ q) : (Γ ⊢ᴵ (p ⟶ q)) := by
   exact dtrAux (insert p Γ) p q d |>.weakening' (by simp);
@@ -107,7 +107,7 @@ instance : Hilbert.HasDT (@Deduction α) := ⟨dtr⟩
 
 def compact {Γ : Theory α} {p} : (Γ ⊢ᴵ p) → (Δ : { Δ : Context α | ↑Δ ⊆ Γ}) × (Δ ⊢ᴵ p)
   | @axm _ Γ p h  => ⟨⟨{p}, by simpa⟩, axm (by simp)⟩
-  | @modus_ponens _ Γ p q h₁ h₂ => by
+  | @modusPonens _ Γ p q h₁ h₂ => by
       have ⟨⟨Δ₁, hs₁⟩, d₁⟩ := h₁.compact;
       have ⟨⟨Δ₂, hs₂⟩, d₂⟩ := h₂.compact;
       simp at hs₁ d₁ hs₂ d₂;
